Skip to content

HTTPS clone URL

Subversion checkout URL

You can clone with HTTPS or Subversion.

Download ZIP
Fetching contributors…

Cannot retrieve contributors at this time

241 lines (173 sloc) 12.732 kb
<!DOCTYPE html>
<html data-require="math mathformat word-problems">
<head>
<title>Age Word Problems</title>
<script src="../khan-exercise.js"></script>
</head>
<body>
<div class="exercise">
<div class="vars">
</div>
<div class="problems">
<div id="solve-older-1">
<div class="vars">
<var id="C">randRange(3, 5)</var>
<var id="B">randRange(2, 20)</var>
<var id="A">randRange(1, 10) * (C - 1)</var>
</div>
<div class="question">
<p><var>person(1)</var> is <var>A</var> years older than
<var>person(2)</var>. <var>B</var> years ago, <var>person(1)</var>
was <var>C</var> times as old as <var>person(2)</var>.</p>
<p>How old is <var>person(1)</var> now?</p>
</div>
<div class="solution"><var>(C * (B + A) - B) / (C - 1)</var></div>
<div class="hints">
<p class="hint1">Let <var>person(1)</var>'s current age be <code><var>personVar(1)</var></code>.</p>
<p class="hint2">That means that <var>B</var> years ago, <var>person(1)</var> was <code><var>personVar(1)</var> - <var>B</var></code> years old.</p>
<p class="hint3"><var>person(2)</var> is <code><var>personVar(1)</var> - <var>A</var></code> years old right now, so <var>B</var> years ago, <var>he(2)</var> was <code>(<var>personVar(1)</var> - <var>A</var>) - <var>B</var> = <var>personVar(1)</var> - <var>A + B</var></code> years old.</p>
<p class="hint4"><var>person(1)</var> was <var>C</var> times as old as <var>person(2)</var>, so that means <code><var>personVar(1)</var> - <var>B</var> = <var>C</var> (<var>personVar(1)</var> - <var>A + B</var>)</code>.</p>
<p class="hint5">Expand: <code><var>personVar(1)</var> - <var>B</var> = <var>C</var> <var>personVar(1)</var> - <var>C * (A + B)</var></code>.</p>
<p class="hint6">Solve for <code><var>personVar(1)</var></code> to get <code><var>C - 1</var> <var>personVar(1)</var> = <var>C * (A + B) - B</var></code>; <code><var>personVar(1)</var> = <var>(C * (B + A) - B) / (C - 1)</var></code>.</p>
</div>
</div>
<div id="solve-younger-1" data-type="solve-older-1">
<div class="question">
<p><var>person(1)</var> is <var>A</var> years older than
<var>person(2)</var>. <var>B</var> years ago, <var>person(1)</var>
was <var>C</var> times as old as <var>person(2)</var>.</p>
<p>How old is <var>person(2)</var> now?</p>
</div>
<div class="solution"><var>(A - B + C * B) / (C - 1)</var></div>
<div class="hints">
<p class="hint1">Let <var>person(2)</var>'s current age be <code><var>personVar(2)</var></code>.</p>
<p class="hint2">That means that <var>person(1)</var> is currently <code><var>personVar(2)</var> + <var>A</var></code> years old and <var>B</var> years ago, <var>person(1)</var> was <code>(<var>personVar(2)</var> + <var>A</var>) - <var>B</var> = <var>personVar(2)</var> + <var>A - B</var></code> years old.</p>
<p class="hint3"><var>B</var> years ago, <var>person(2)</var> was <code><var>personVar(2)</var> - <var>B</var></code> years old.</p>
<p class="hint4"><var>person(1)</var> was <var>C</var> times as old as <var>person(2)</var>, so that means <code><var>personVar(2)</var> + <var>A - B</var> = <var>C</var> (<var>personVar(2)</var> - <var>B</var>)</code>.</p>
<p class="hint5">Expand: <code><var>personVar(2)</var> + <var>A - B</var> = <var>C</var> <var>personVar(2)</var> - <var>C * B</var></code>.</p>
<p class="hint6">Solve for <code><var>personVar(2)</var></code> to get <code><var>C - 1</var> <var>personVar(2)</var> = <var>A - B + C * B</var></code>; <code><var>personVar(2)</var> = <var>(A - B + C * B) / (C - 1)</var></code>.</p>
</div>
</div>
<div id="solve-older-2">
<div class="vars">
<var id="C">randRange(3, 5)</var>
<var id="A">randRange(2, 10) * (C - 1)</var>
</div>
<div class="question">
<p><var>person(1)</var> is <var>C</var> times as old as
<var>person(2)</var> and is also <var>A</var>
years older than <var>person(2)</var>.</p>
<p>How old is <var>person(1)</var>?</p>
</div>
<div class="solution"><var>A * C / (C - 1)</var></div>
<div class="hints">
<p class="hint1">Let <var>person(1)</var>'s age be <code><var>personVar(1)</var></code>.</p>
<p class="hint2">We know <var>person(2)</var> is <code>1/<var>C</var></code> as old as <var>person(1)</var>, so <var>person(2)</var>'s age can be written as <code><var>personVar(1)</var> / <var>C</var></code>.</p>
<p class="hint3"><var>His(2)</var> age can also be written as <code><var>personVar(1)</var> - <var>A</var></code>.</p>
<p class="hint4">Set the two expressions for <var>person(2)</var>'s age equal to each other: <code><var>personVar(1)</var> / <var>C</var> = <var>personVar(1)</var> - <var>A</var></code>.</p>
<p class="hint5">Multiply both sides by <code><var>C</var></code> to get <code><var>personVar(1)</var> = <var>C</var> <var>personVar(1)</var> - <var>A * C</var></code>.</p>
<p class="hint6">Solve for <code><var>personVar(1)</var></code> to get <code><var>C - 1</var> <var>personVar(1)</var> = <var>A * C</var></code>; <code><var>personVar(1)</var> = <var>A * C / (C - 1)</var></code>.</p>
</div>
</div>
<div id="solve-younger-2" data-type="solve-older-2">
<div class="question">
<p><var>person(1)</var> is <var>C</var> times as old as
<var>person(2)</var> and is also <var>A</var>
years older than <var>person(2)</var>.</p>
<p>How old is <var>person(2)</var>?</p>
</div>
<div class="solution"><var>A / (C - 1)</var></div>
<div class="hints">
<p class="hint1">Let <var>person(2)</var>'s age be <code><var>personVar(2)</var></code>.</p>
<p class="hint2">We know <var>person(1)</var> is <var>C</var> times as old as <var>person(2)</var>, so <var>person(1)</var>'s age can be written as <code><var>C</var> <var>personVar(2)</var></code>.</p>
<p class="hint3"><var>His(1)</var> age can also be written as <code><var>personVar(2)</var> + <var>A</var></code>.</p>
<p class="hint4">Set the two expressions for <var>person(1)</var>'s age equal to each other: <code><var>C</var> <var>personVar(2)</var> = <var>personVar(2)</var> + <var>A</var></code>.</p>
<p class="hint5">Solve for <code><var>personVar(2)</var></code> to get <code><var>C - 1</var> <var>personVar(2)</var> = <var>A</var></code>; <code><var>personVar(2)</var> = <var>A / (C - 1)</var></code>.</p>
</div>
</div>
<div id="solve-older-3">
<div class="vars">
<var id="A">randRange(2, 5)</var>
<var id="C" data-ensure="C - A !== A">randRange(A + 2, 9)</var>
<var id="B">randRange(2, 10) * (C - A)</var>
</div>
<div class="question">
<p><var>person(1)</var> is <var>A</var> times as old as <var>person(2)</var>. <var>B</var> years ago, <var>person(1)</var> was <var>C</var> times as old as <var>person(2)</var>.</p>
<p>How old is <var>person(1)</var> now?</p>
</div>
<div class="solution"><var>A * B * (C - 1) / (C - A)</var></div>
<div class="hints">
<p class="hint1">Let <var>person(1)</var>'s age be <code><var>personVar(1)</var></code>.</p>
<p class="hint2">We know <var>person(2)</var> is <code>1/<var>A</var></code> as old as <var>person(1)</var>, so <var>person(2)</var>'s age can be written as <code><var>personVar(1)</var> / <var>A</var></code>.</p>
<p class="hint3"><var>B</var> years ago, <var>person(1)</var> was <code><var>personVar(1)</var> - <var>B</var></code> years old and <var>person(2)</var> was <code><var>personVar(1)</var> / <var>A</var> - <var>B</var></code> years old.</p>
<p class="hint4">At that time, <var>person(1)</var> was <var>C</var> times as old as <var>person(2)</var>, so we can write <code><var>personVar(1)</var> - <var>B</var> = <var>C</var> (<var>personVar(1)</var> / <var>A</var> - <var>B</var>)</code>.</p>
<p class="hint5">Expand: <code><var>personVar(1)</var> - <var>B</var> = <var>fraction(C, A)</var> <var>personVar(1)</var> - <var>C * B</var></code>.</p>
<p class="hint6">Solve for <code><var>personVar(1)</var></code> to get <code><var>fraction(C - A, A)</var> <var>personVar(1)</var> = <var>B * (C - 1)</var></code>; <code><var>personVar(1)</var> = <var>fraction(A, C - A)</var> \cdot <var>B * (C - 1)</var> = <var>A * B * (C - 1) / (C - A)</var></code>.</p>
</div>
</div>
<div id="solve-younger-3" data-type="solve-older-3">
<div class="question">
<p><var>person(1)</var> is <var>A</var> times as old as <var>person(2)</var>. <var>B</var> years ago, <var>person(1)</var> was <var>C</var> times as old as <var>person(2)</var>.</p>
<p>How old is <var>person(2)</var> now?</p>
</div>
<div class="solution"><var>B * (C - 1) / (C - A)</var></div>
<div class="hints">
<p class="hint1">Let <var>person(2)</var>'s age be <code><var>personVar(2)</var></code>.</p>
<p class="hint2">We know <var>person(1)</var> is <var>A</var> times as old as <var>person(2)</var>, so <var>person(1)</var>'s age can be written as <code><var>A</var> <var>personVar(2)</var></code>.</p>
<p class="hint3"><var>B</var> years ago, <var>person(1)</var> was <code><var>A</var> <var>personVar(2)</var> - <var>B</var></code> years old and <var>person(2)</var> was <code><var>personVar(2)</var> - <var>B</var></code> years old.</p>
<p class="hint4">At that time, <var>person(1)</var> was <var>C</var> times as old as <var>person(2)</var>, so we can write <code><var>A</var> <var>personVar(2)</var> - <var>B</var> = <var>C</var> (<var>personVar(2)</var> - <var>B</var>)</code>.</p>
<p class="hint5">Expand: <code><var>A</var> <var>personVar(2)</var> - <var>B</var> = <var>C</var> <var>personVar(2)</var> - <var>B * C</var></code>.</p>
<p class="hint6">Solve for <code><var>personVar(1)</var></code> to get <code><var>C - A</var> <var>personVar(1)</var> = <var>B * (C - 1)</var></code>; <code><var>personVar(1)</var> = <var>B * (C - 1) / (C - A)</var></code>.</p>
</div>
</div>
<div id="solve-single-4" data-weight="2">
<div class="vars">
<var id="A">randRange(3, 20)</var>
<var id="B" data-ensure="B <= 60">randRange(7, 24) * (A - 1)</var>
</div>
<div class="question">
<p>In <var>B</var> years, <var>person(1)</var> will be <var>A</var> times as old as <var>he(1)</var> is right now.</p>
<p>How old is <var>he(1)</var> right now?</p>
</div>
<div class="solution"><var>B / (A - 1)</var></div>
<div class="hints">
<p class="hint1">Let <var>person(1)</var>'s age be <code><var>personVar(1)</var></code>.</p>
<p class="hint2">In <var>B</var> years, <var>he(1)</var> will be <code><var>personVar(1)</var> + <var>B</var></code> years old.</p>
<p class="hint3">At that time, <var>he(1)</var> will also be <code><var>A</var> <var>personVar(1)</var></code> years old.</p>
<p class="hint4">We write <code><var>personVar(1)</var> + <var>B</var> = <var>A</var> <var>personVar(1)</var></code>.</p>
<p class="hint5">Solve for <code><var>personVar(1)</var></code> to get <code><var>A - 1</var> <var>personVar(1)</var> = <var>B</var></code>; <code><var>personVar(1)</var> = <var>B / (A - 1)</var></code>.</p>
<p class="hint6"></p>
</div>
</div>
<div id="solve-single-5" data-weight="2">
<div class="vars">
<var id="C">randRange(3, 5)</var>
<var id="B" data-ensure="B > 1.5">randRange(1, 10) * (C - 1)</var>
<var id="A" data-ensure="A <= 80">randRange(C * B + 1, 15) * (C - 1)</var>
</div>
<div class="question">
<p><var>person(1)</var> is <var>A</var> years old and <var>person(2)</var> is <var>B</var> years old.</p>
<p>How many years will it take until <var>person(1)</var> is only <var>C</var> times as old as <var>person(2)</var>?</p>
</div>
<div class="solution"><var>(A - B * C) / (C - 1)</var></div>
<div class="hints">
<p class="hint1">Let <code>y</code> be the number of years that it will take.</p>
<p class="hint2">In <code>y</code> years, <var>person(1)</var> will be <code><var>A</var> + y</code> years old and <var>person(2)</var> will be <code><var>B</var> + y</code> years old.</p>
<p class="hint3">At that time, <var>person(1)</var> will be <var>C</var> times as old as <var>person(2)</var>.</p>
<p class="hint4">We write <code><var>A</var> + y = <var>C</var> (<var>B</var> + y)</code>.</p>
<p class="hint5">Expand to get <code><var>A</var> + y = <var>C * B</var> + <var>C</var> y</code>.</p>
<p class="hint6">Solve for <code>y</code> to get <code><var>C - 1</var> y = <var>A - C * B</var></code>; <code>y = <var>(A - C * B) / (C - 1)</var></code>.</p>
</div>
</div>
</div>
<div class="hints">
<p class="hint1"></p>
<p class="hint2"></p>
<p class="hint3"></p>
<p class="hint4"></p>
<p class="hint5"></p>
<p class="hint6"></p>
</div>
</div>
</body>
</html>
Jump to Line
Something went wrong with that request. Please try again.